layout of the field structure

code/bignum/Hacl.Spec.Bignum.fst
@@ -18,31 +18,75 @@ module U32 = FStar.UInt32
 module F   = Hacl.Spec.Bignum.Field
 
 
-#set-options "--initial_fuel 0 --max_fuel 0"
+(* Prime field definitions *)
 
-val fsum_tot: a:seqelem{red a len} -> b:seqelem{red b len} -> Tot (c:seqelem)
+type elem = e:int{e >= 0 /\ e < prime}
+
+let zero : elem = 0
+let one  : elem = 1
+
+val fadd: elem -> elem -> Tot elem
+let fadd e1 e2 = (e1 + e2) % prime
+let op_Plus_At e1 e2 = fadd e1 e2
+
+val fdiff: elem -> elem -> Tot elem
+let fdiff e1 e2 = (e1 - e2) % prime
+let op_Subtraction_At e1 e2 = fdiff e1 e2
+
+val fmul: elem -> elem -> Tot elem
+let fmul e1 e2 = (e1 * e2) % prime
+let op_Star_At e1 e2 = fmul e1 e2
+
+val selem: seqelem -> GTot elem
+let selem s = seval s % prime
+
+assume val lemma_mod_sub_distr_l_l: a:nat -> b:nat -> p:pos -> Lemma ((a - b) % p = ((a % p) - b) % p)
+assume val lemma_mod_sub_distr_l_r: a:nat -> b:nat -> p:pos -> Lemma ((a - b) % p = (a - (b % p)) % p)
+
+
+#reset-options "--initial_fuel 0 --max_fuel 0 --z3rlimit 20"
+
+val fsum_tot:
+  a:seqelem{red a len} ->
+  b:seqelem{red b len} ->
+  Tot (c:seqelem{selem c = selem a +@ selem b})
 let fsum_tot a b =
-  fsum_spec a b len
+  Math.Lemmas.lemma_mod_plus_distr_l (seval a) (seval b) prime;
+  Math.Lemmas.lemma_mod_plus_distr_l (seval b) (selem a) prime;
+  let c = fsum_spec a b len in
+  lemma_fsum_eval a b;
+  c
 
 
-#set-options "--z3rlimit 20"
+#reset-options "--initial_fuel 0 --max_fuel 0 --z3rlimit 20"
 
 val fdifference_tot:
-  a:seqelem -> b:seqelem{add_zero_pre b /\ gte_limbs a (add_zero_spec b) len} -> Tot seqelem
+  a:seqelem ->
+  b:seqelem{add_zero_pre b /\ gte_limbs a (add_zero_spec b) len} ->
+  Tot (c:seqelem{selem c = selem b -@ selem a})
 let fdifference_tot a b =
   let b' = add_zero_spec b in
-  fdifference_spec a b' len
+  lemma_add_zero_spec b;
+  let c = fdifference_spec a b' len in
+  lemma_fdifference_eval a b';
+  lemma_mod_sub_distr_l_l (seval b') (seval a) prime;
+  lemma_mod_sub_distr_l_r (selem b') (seval a) prime;
+  c
 
+open FStar.Mul
 
 val fscalar_tot: a:seqelem -> s:limb{
   carry_wide_pre (fscalar_spec a s) 0
   /\ carry_top_wide_pre (carry_wide_spec (fscalar_spec a s) 0)
   /\ copy_from_wide_pre (carry_top_wide_spec (carry_wide_spec (fscalar_spec a s) 0)) } ->
-  Tot seqelem
+  (* Tot (c:seqelem{selem c = (v s * selem a) % prime}) *)
+  Tot (c:seqelem)
 let fscalar_tot a s =
   let x = fscalar_spec a s in
-  let y = carry_wide_spec x 0 in  
+  lemma_fscalar_eval a s;
+  let y = carry_wide_spec x 0 in
   let z = carry_top_wide_spec y in
+  lemma_carry_top_wide_spec y;
   copy_from_wide_spec z
 
 
